theories/Compositional_Structures/Basic_Modules/Component_Types/Defer_Equal_Condition_Ref.thy
@@ -20,15 +20,14 @@ text \<open>
 
 subsection \<open>Definition\<close>
 
-lemma op_repl: "card = op_set_size"
-  by auto
-
+lemma card_is_set_size: "card = op_set_size"
+  by simp
 
 sepref_definition defer_equal_condition_sep is "uncurry (RETURN oo defer_equal_condition)" ::
 "nat_assn\<^sup>k *\<^sub>a result_impl_assn\<^sup>k \<rightarrow>\<^sub>a bool_assn"
-  unfolding defer_equal_condition.simps
-  apply (rewrite in "_ \<hole>" op_repl)
-  apply sepref_dbg_keep
-  done
+  unfolding defer_equal_condition.simps card_is_set_size
+  by sepref
+
+thm "defer_equal_condition_sep.refine"
 
 end
