theories/Compositional_Structures/Sepref_Bindings.thy
@@ -1,38 +1,58 @@
 theory Sepref_Bindings
   imports "Basic_Modules/Borda_Module_Ref"
-    "Basic_Modules/Condorcet_Module_Ref"
+    "Basic_Modules/Condorcet_Module_Ref"  
+    "Basic_Modules/Component_Types/Defer_Equal_Condition_Ref"
     Sequential_Composition_Ref
 
 begin
 
-
-
-sepref_decl_op (no_def) borda_mod: "borda_ref :: 'a Electoral_Module_Ref" :: "elec_mod_rel_ref Id"
+lemma borda_aux:
+  shows "(uncurry (RETURN \<circ>\<circ> borda), uncurry (RETURN \<circ>\<circ> borda))
+    \<in> \<langle>Id\<rangle>set_rel \<times>\<^sub>r
+       \<langle>\<langle>Id \<times>\<^sub>r Id\<rangle>set_rel\<rangle>list_rel \<rightarrow>\<^sub>f \<langle>\<langle>Id\<rangle>set_rel \<times>\<^sub>r \<langle>Id\<rangle>set_rel \<times>\<^sub>r \<langle>Id\<rangle>set_rel\<rangle>nres_rel"
   apply standard
   apply (rule nres_relI)
   apply simp
   done
 
-sepref_decl_op (no_def) borda_doit: "borda :: 'a Electoral_Module" :: "elec_mod_rel_orig Id"
+lemma condorcet_aux:
+  shows "(uncurry (RETURN \<circ>\<circ> condorcet), uncurry (RETURN \<circ>\<circ> condorcet))
+    \<in> \<langle>Id\<rangle>set_rel \<times>\<^sub>r
+       \<langle>\<langle>Id \<times>\<^sub>r Id\<rangle>set_rel\<rangle>list_rel \<rightarrow>\<^sub>f \<langle>\<langle>Id\<rangle>set_rel \<times>\<^sub>r \<langle>Id\<rangle>set_rel \<times>\<^sub>r \<langle>Id\<rangle>set_rel\<rangle>nres_rel"
   apply standard
   apply (rule nres_relI)
   apply simp
   done
-  
 
-  context 
-    notes alts_assn_def[symmetric,fcomp_norm_unfold] 
-       profile_assn_def[symmetric,fcomp_norm_unfold]
+
+sepref_decl_op (no_def) "borda :: 'a Electoral_Module" :: "elec_mod_rel_orig_nres Id" 
+  using borda_aux .
+
+(*sepref_decl_op (no_def) "condorcet :: 'a Electoral_Module" :: "elec_mod_rel_orig_nres Id"
+  apply standard
+  apply (rule nres_relI)
+  apply simp 
+  done*)
+
+sepref_decl_op (no_def) defer_equal_imp: "(defer_equal_condition)" :: 
+  "\<langle>nat_rel, \<langle>(\<langle>R\<rangle>set_rel \<times>\<^sub>r \<langle>R\<rangle>set_rel \<times>\<^sub>r \<langle>R\<rangle>set_rel), \<langle>bool_rel\<rangle>nres_rel\<rangle>fun_rel\<rangle>fun_rel" 
+  where "R = Id" .
+
+locale refine_assns =
+ notes  
+       ballot_assn_def[symmetric,fcomp_norm_unfold]
        result_set_assn_def[symmetric,fcomp_norm_unfold]
- alts_ref_assn_def[symmetric,fcomp_norm_unfold] ballot_ref_assn_def[symmetric,fcomp_norm_unfold]
+       alts_ref_assn_def[symmetric,fcomp_norm_unfold] ballot_ref_assn_def[symmetric,fcomp_norm_unfold]
+       alts_assn_def[symmetric,fcomp_norm_unfold] 
+       result_set_one_step_def[symmetric,fcomp_norm_unfold]
       
 begin
 
+thm borda_elim_sepref.refine[FCOMP borda_ref_correct]
 
-sepref_decl_impl borda_impl: borda_elim_sepref.refine[FCOMP borda_ref_correct] 
-  unfolding alts_ref_assn_def .
+sepref_decl_impl borda_impl: borda_elim_sepref.refine[FCOMP borda_ref_correct]  .
 
+sepref_decl_impl defer_eqal_condition_impl: defer_equal_condition_sep.refine .
 
-
-                                                
 end
+
